\documentclass[a4paper,12pt]{article}
%%%%%%%%%%%%%%%%%%%%%%%%%%%%%%%%%%%%%%%%%%%%%%%%%%%%%%%%%%%%%%%%%%%%%%%%%%%%%%%%%%%%%%%%%%%%%%%%%%%%%%%%%%%%%%%%%%%%%%%%%%%%%%%%%%%%%%%%%%%%%%%%%%%%%%%%%%%%%%%%%%%%%%%%%%%%%%%%%%%%%%%%%%%%%%%%%%%%%%%%%%%%%%%%%%%%%%%%%%%%%%%%%%%%%%%%%%%%%%%%%%%%%%%%%%%%
\usepackage{eurosym}
\usepackage{vmargin}
\usepackage{amsmath}
\usepackage{framed}
\usepackage{multicol}
\usepackage{graphics}
\usepackage{epsfig}
\usepackage{subfigure}
\usepackage{enumerate}
\usepackage{fancyhdr}

\setcounter{MaxMatrixCols}{10}
%TCIDATA{OutputFilter=LATEX.DLL}
%TCIDATA{Version=5.00.0.2570}
%TCIDATA{<META NAME="SaveForMode"CONTENT="1">}
%TCIDATA{LastRevised=Wednesday, February 23, 201113:24:34}
%TCIDATA{<META NAME="GraphicsSave" CONTENT="32">}
%TCIDATA{Language=American English}

\pagestyle{fancy}
\setmarginsrb{20mm}{0mm}{20mm}{25mm}{12mm}{11mm}{0mm}{11mm}
\lhead{MathsResource} \chead{Calculus} \rhead{Differentiation} %\input{tcilatex}
\begin{document}
\section*{Differentiation}

\begin{enumerate}
\item Differentiate $f(x)$ with respect to $x$ for each of the following cases:
	\begin{multicols}{2}
		\begin{enumerate}[(a)]
			\item	\qquad	 $ f(x) = x^2 \,$ %%%={{noprint|ˆt2x</math>}}}}
			\item	\qquad	 $ f(x) = 2x + 2 \,$ %%%={{noprint|ˆt2</math>}}}}
			\item	\qquad	 $ f(x) = \frac{1}{2}x^2 \,$ %%%={{noprint|ˆtx</math>}}}}
			\item	\qquad	 $ f(x) = 2x^2 + 4x + 4 \,$ %%%={{noprint|ˆt4x+4</math>}}}}

			\item	\qquad	 $ f(x) = \sqrt{x+2} \,$
			%%%={{noprint|ˆt\frac{1}{2\sqrt{x+2}}</math>}}}}
								\end{enumerate}
			\end{multicols}
\item Differentiate $f(x)$ with respect to $x$ for each of the following cases:			
				\begin{multicols}{2}
		\begin{enumerate}[(a)]
		\item		 $ \displaystyle{ f(x) = \frac{1}{x} \,}$ %%%={{noprint|ˆt-\frac{1}{x^2}</math>}}}}
			\item		 $ \displaystyle{ f(x) = \frac{3}{x+1} \,}$ %%%={{noprint|ˆt\frac{-3}{(x+1)^2}</math>}}}}
			\item		 $ \displaystyle{ f(x) = \frac{1}{\sqrt{x+1}} \,}$ %%%={{noprint|ˆt\frac{-1}{2(x+1)^{3/2}}</math>}}}}
				\item		 $ \displaystyle{ f(x) = \frac{x}{x+2} \,}$ %%%={{noprint|ˆt\frac{2}{(x+2)^2}</math>}}}}
				\end{enumerate}
			\end{multicols}
			

% \subsubsection*{Selected Solutions}
%\begin{framed}	
%
%	\begin{multicols}{2}
%		\begin{enumerate}[(a)]
%			\item	\qquad	 $ 2x$			\item	\qquad	 $2$
%			\item	\qquad	 $ x$
%			\item	\qquad	 $ 4x+4$ \\
%			\item		 $ \displaystyle{ \frac{1}{2\sqrt{x+2}}}$
%			\item		 $ \displaystyle{ -\frac{1}{x^2}}$
%			\item		 $ \displaystyle{ \frac{-3}{(x+1)^2}}$
%			\item $ \displaystyle{\frac{-1}{2(x+1)^{3/2}}}$
%			\item		$ \displaystyle{\frac{2}{(x+2)^2}}$
%		\end{enumerate}
%	\end{multicols}
%\end{framed}
%\newpage
\item Differentiate $f(x)$ with respect to $x$ for each of the following cases:
				\begin{multicols}{2}
					\begin{enumerate}[(a)]
						
						\item		 $ \displaystyle{ f(x) = 2x^2 + 4\,}$ %%%={{noprint|ˆtf'(x)=4x</math>}}}}
						\item		 $ \displaystyle{ f(x) = 3\sqrt[3]{x}\, }$
						\item		 $ \displaystyle{ f(x) = 2x^5+8x^2+x-78\,}$ %%%={{noprint|ˆtf'(x)=10x^4+16x+1</math>}}}}
						\item		 $ \displaystyle{ f(x) = 7x^7+8x^5+x^3+x^2-x\,}$ %%%={{noprint|ˆtf'(x)=49x^6+40x^4+3x^2+2x-1</math>}}}}
						\item		$ \displaystyle{ f(x) = \frac{1}{x^2}+3x^\frac{1}{3}\,}$ %%%={{noprint|ˆtf'(x)=\frac{-2}{x^3}+\frac{1}{\sqrt[3]{x^2}}</math>}}}}
					\end{enumerate}
				\end{multicols}
\item Differentiate $f(x)$ with respect to $x$ for each of the following cases:
				\begin{multicols}{2}
					\begin{enumerate}[(a)]				
						\item		 $ \displaystyle{ f(x) = 3x^{15} + \frac{1}{17}x^2 +\frac{2}{\sqrt{x}} \,}$ %%%={{noprint|ˆtf'(x)=45x^{14}+\frac{2}{17}x-\frac{1}{x\sqrt{x}}</math>}}}}
						\item		 $ \displaystyle{ f(x) = \frac{3}{x^4} - \sqrt[4]{x} + x \,}$ %%%={{noprint|ˆtf'(x)=\frac{-12}{x^5}-\frac{1}{4\sqrt[4]{x^3}}+1</math>}}}}
						\item		 $ \displaystyle{ f(x) = 6x^{1/3}-x^{0.4} +\frac{9}{x^2} \,}$ %%%={{noprint|ˆtf'(x)=\frac{2}{\sqrt[3]{x^2}}-\frac{0.4}{x^{0.6}}-\frac{18}{x^3}</math>}}}}
						\item		 $ \displaystyle{ f(x) = \frac{1}{\sqrt[3]{x}} + \sqrt{x} \,}$ %%%={{noprint|ˆtf'(x)=\frac{-1}{3x\sqrt[3]{x}}+\frac{1}{2\sqrt{x}}</math>}}}}
					\end{enumerate}
				\end{multicols}
				
\end{enumerate}				
\end{document}
