\documentclass[a4paper,12pt]{article}
%%%%%%%%%%%%%%%%%%%%%%%%%%%%%%%%%%%%%%%%%%%%%%%%%%%%%%%%%%%%%%%%%%%%%%%%%%%%%%%%%%%%%%%%%%%%%%%%%%%%%%%%%%%%%%%%%%%%%%%%%%%%%%%%%%%%%%%%%%%%%%%%%%%%%%%%%%%%%%%%%%%%%%%%%%%%%%%%%%%%%%%%%%%%%%%%%%%%%%%%%%%%%%%%%%%%%%%%%%%%%%%%%%%%%%%%%%%%%%%%%%%%%%%%%%%%
\usepackage{eurosym}
\usepackage{vmargin}
\usepackage{amsmath}
\usepackage{framed}
\usepackage{graphics}
\usepackage{epsfig}
\usepackage{subfigure}
\usepackage{enumerate}
\usepackage{fancyhdr}
\usepackage{multicol}

\setcounter{MaxMatrixCols}{10}
%TCIDATA{OutputFilter=LATEX.DLL}
%TCIDATA{Version=5.00.0.2570}
%TCIDATA{<META NAME="SaveForMode"CONTENT="1">}
%TCIDATA{LastRevised=Wednesday, February 23, 201113:24:34}
%TCIDATA{<META NAME="GraphicsSave" CONTENT="32">}
%TCIDATA{Language=American English}

\pagestyle{fancy}
\setmarginsrb{20mm}{0mm}{20mm}{25mm}{12mm}{11mm}{0mm}{11mm}
\lhead{MathsResource} \chead{Calculus} \rhead{Functions of Several Variables} %\input{tcilatex}
\begin{document}

\subsection*{Functions of Several Variables : Tutorial Sheet 1}

\begin{enumerate}
    \item  Evaluate all the first partial derivatives, i.e. $\frac{\partial z}{\partial x}$ and $\frac{\partial z}{\partial y} $, 
of the following function:

\[ z = 2xy^3 + \cos(2x) - \sin(y) .\]



 \item 
 Show that the function $z=e^{-2t}\cos(x)$ satisfied the partial differential equation
 \[ 4\frac{\partial^2 z}{\partial x^2} + \frac{\partial^2 z}{\partial t^2} = 0. \]
 
 
 
 \item Determine both of the first order partial derivatives with respect to $z$ of the following expression.

\[ z = \frac{x^2y^3}{3} +  y \cos(x)\]
 

	\item Find $\displaystyle{ \frac{ \partial^2 z }{ \partial^2 x  }}$ and $\displaystyle{ \frac{ \partial^2 z }{ \partial^2 y }}$  for the following function
\[ z = x^2y + 3x^2y^3 - 9x^2.\]	

	\item	Show that the function $z=e^{-3y}\cos(x)$ satisfies the partial differential equation
	\[ 9\frac{\partial^2 z}{\partial x^2} + \frac{\partial^2 z}{\partial y^2} = 0. \]


	
	
	\item Find $\displaystyle{ \frac{ \partial^2 z }{ \partial x^2 }}$ and $\displaystyle{ \frac{ \partial^2 z }{ \partial y^2 }}$  for both of the following functions:
%	\[ z = 3x^2y^3 + y\cosh(x) - 9y^2 +10x^3.\]	

	\begin{multicols}{2}
		\begin{itemize}
			\item[(a)] $\displaystyle{  z = 9y^2 +10x^3. }  $
				\item[(b)] $\displaystyle{  z = 3x^2y^3 + y\cosh(x).}$
				
			\end{itemize}
		\end{multicols}

\item 
	Show that the function $z=e^{-4y}\cos(x)$ satisfies the partial differential equation
	\[ 16\frac{\partial^2 z}{\partial x^2} + \frac{\partial^2 z}{\partial y^2} = 0. \]
	
\item Evaluate all the first partial derivatives, i.e. $\frac{\partial z}{\partial x}$ and $\frac{\partial z}{\partial y} $, 
of the following function:

\[ z = 2xy^3 + \cos(2x) - \sin(y) \]

 \item 
 Show that the function $z=e^{2t}\sin(4x)$ satisfied the partial differential equation
 \[ \frac{\partial^2 z}{\partial x^2} +  4\frac{\partial^2 z}{\partial t^2} = 0. \]


\end{enumerate}
\end{document}

