**Exam Question:**

**Question:**

**a)** Find the Laplace transform of the following function:

$$$
f(t) = t^2 * e^(-3t) * sin(2t)
$$$

**b)** Solve the following differential equation using the Laplace transform method:

$$$
y'' + 4y' + 3y = e^(-2t)
$$$

**Initial conditions:**
* y(0) = 0
* y'(0) = 1

**Solution:**

**a) Laplace Transform of f(t)**

We can use the following Laplace transform properties:

* **Time-shifting property:** L{e^(-at)f(t)} = F(s+a)
* **Differentiation in s-domain:** L{t^nf(t)} = (-1)^n * F^(n)(s)
* **Laplace transform of sin(ωt):** L{sin(ωt)} = ω / (s^2 + ω^2)

Applying these properties, we get:
$$$
L{t^2 * e^(-3t) * sin(2t)} = (-1)^2 * d^2/ds^2 [2 / ((s+3)^2 + 4)]
$$$
Now, differentiate and simplify to obtain the final Laplace transform.

**b) Solving the Differential Equation**

1. **Take the Laplace Transform of both sides:**

$$$
s^2Y(s) - s*y(0) - y'(0) + 4[sY(s) - y(0)] + 3Y(s) = 1 / (s+2)
$$$

2. **Substitute initial conditions and simplify:**
$$$
(s^2 + 4s + 3)Y(s) = 1 / (s+2) + 1
$$$

3. **Solve for Y(s):**
$$$
Y(s) = (s+3) / [(s+1)(s+2)(s+3)]
$$$

4. **Partial Fraction Decomposition:**
$$$
Y(s) = A/(s+1) + B/(s+2)
$$$
Solve for A and B.

5. **Inverse Laplace Transform:**
Use the inverse Laplace transform table to find the solution y(t).
$$$
y(t) = A*e^(-t) + B*e^(-2t)
$$$
Substitute the values of A and B to get the final solution.
